practice.v
@@ -2,6 +2,7 @@ Require Import Coq.Arith.Arith.
 Require Import Coq.Arith.PeanoNat.
 Require Import Coq.Arith.Even.
 
+Require Import AbstractState.
 Require Import AbstractInterpreter.
 Require Import Aux.
 Require Import ConcreteInterpreter.
@@ -16,76 +17,58 @@ Definition abstract_state := total_map (parity).
 Open Scope com_scope.
 
 Lemma abstract_aexp_plus_sound : forall st ast e1 e2,
-  gamma (abstract_eval_aexp ast e1) (eval_aexp st e1) ->
-  gamma (abstract_eval_aexp ast e2) (eval_aexp st e2) ->
-  gamma (abstract_eval_aexp ast (APlus e1 e2)) (eval_aexp st (APlus e1 e2)).
+  gamma_par (abstract_eval_aexp ast e1) (eval_aexp st e1) ->
+  gamma_par (abstract_eval_aexp ast e2) (eval_aexp st e2) ->
+  gamma_par (abstract_eval_aexp ast (APlus e1 e2)) (eval_aexp st (APlus e1 e2)).
 Proof.
   intros. simpl. apply gamma_distr_plus; assumption.
 Qed.
 
 Lemma abstract_aexp_mult_sound : forall ast st e1 e2,
-  gamma (abstract_eval_aexp ast e1) (eval_aexp st e1) ->
-  gamma (abstract_eval_aexp ast e2) (eval_aexp st e2) ->
-  gamma (abstract_eval_aexp ast (AMult e1 e2)) (eval_aexp st (AMult e1 e2)).
+  gamma_par (abstract_eval_aexp ast e1) (eval_aexp st e1) ->
+  gamma_par (abstract_eval_aexp ast e2) (eval_aexp st e2) ->
+  gamma_par (abstract_eval_aexp ast (AMult e1 e2)) (eval_aexp st (AMult e1 e2)).
 Proof. intros. simpl. apply gamma_distr_mult; assumption.
 Qed.
 
 Lemma abstract_aexp_var_sound : forall ast st x,
-  gamma (ast x) (st x) -> 
-  gamma (abstract_eval_aexp ast (AVar x)) (eval_aexp st (AVar x)).
-Proof. intros. simpl. assumption. Qed.
+  sound_state ast st ->
+  gamma_par (abstract_eval_aexp ast (AVar x)) (eval_aexp st (AVar x)).
+Proof. intros. simpl. auto. Qed.
 
-Theorem abstract_aexp_eval_sound : forall ast x st e,
-  gamma (ast x) (st x) ->
-  (gamma (abstract_eval_aexp ast e)) (eval_aexp st e).
+Theorem abstract_aexp_eval_sound : forall ast st e,
+  sound_state ast st ->
+  (gamma_par (abstract_eval_aexp ast e)) (eval_aexp st e).
 Proof.
   induction e; intros.
   - (* ANum *) simpl. apply gamma_extract_n_n.
-  - (* AVar *) apply abstract_aexp_var_sound. admit.
+  - (* AVar *) apply abstract_aexp_var_sound. apply H.
 
   - (* APlus *) apply abstract_aexp_plus_sound; auto.
   - (* AMult *) apply abstract_aexp_mult_sound; auto.
-Admitted.
-
-Lemma abstract_ceval_ass_sound : forall ast x st a,
-  gamma (ast x) (st x) ->
-  gamma (ceval_abstract ast (x ::= a) x) (ceval st (x ::= a) x).
-Proof.
-  intros. simpl. unfold t_update.  rewrite <- beq_string_refl.
-  apply abstract_aexp_eval_sound with (x:=x). assumption.
 Qed.
 
-Lemma abstract_ceval_seq_sound : forall ast c1 c2 x st,
-  gamma ((ceval_abstract ast c1) x) ((ceval st c1) x) ->
-  gamma (ceval_abstract ast (c1;; c2) x) (ceval st (c1;; c2) x).
+Lemma abstract_ceval_ass_sound : forall ast st y a,
+  sound_state ast st ->
+  sound_state (ceval_abstract ast (y ::= a)) (ceval st (y ::= a)).
 Proof.
-  intros. generalize dependent c1. induction c2; intros.
-  - (* CSkip *) simpl. apply H.
-  - (* CSeq  *) replace (ceval_abstract ast (c1;; c2_1;; c2_2)) with
-    (ceval_abstract ast ((c1;; c2_1);;c2_2)); try reflexivity. 
-    replace (ceval st (c1;; c2_1 ;; c2_2)) with
-      (ceval st ((c1 ;; c2_1) ;; c2_2)); try reflexivity.
-      apply IHc2_2.  apply IHc2_1. apply H.
-  - (* CAss *) simpl. admit.
-Admitted.
+  intros. simpl. unfold t_update, sound_state. intros.
+  destruct (beq_string y x). 
+  - apply abstract_aexp_eval_sound. apply H.
+  - unfold sound_state in H. apply H.
+Qed.
 
-Theorem abstract_ceval_sound : forall ast st c x,
-  (forall x, gamma (ast x) (st x)) ->
-  (gamma ((ceval_abstract ast c) x)) ((ceval st c) x).
+Theorem abstract_ceval_sound : forall ast st c,
+  sound_state ast st ->
+  sound_state (ceval_abstract ast c) (ceval st c).
 Proof.
-  intros. induction c.
-  - (* SKIP *)
-    intros. simpl. apply H.
-  - (* CSeq *)
-    apply abstract_ceval_seq_sound. assumption.
-  - admit.
-Admitted.
-    
-
-
-(* proof the equivalance of the galois connection diagram *)
-(* Peval o gamma \subset gamma o abstract_eval *)
-(* etc... *)
+  unfold sound_state. intros ast st c. revert ast st.
+  induction c.
+  - (* SKIP *) auto.
+  - (* CSeq *) simpl. intros.
+    apply IHc2. clear IHc2. intros. apply IHc1. apply H.
+  - intros. apply abstract_ceval_ass_sound. unfold sound_state. apply H.
+Qed.
 
 (* Add a statements SKIP, sequencing, if statements, assignment *)
 
